<?xml version="1.0" encoding="UTF-8"?>
<section xml:id="s_algebraic" xmlns:xi="http://www.w3.org/2001/XInclude">
	<title>Algebraic extensions</title>
	<definition xml:id="d_fin_gen">
		<title>Finitely generated</title>
		<statement>
			<p>
				Let <m>K/F</m> be a field extension.
				We say <m>K</m> is <term>finitely generated</term> over <m>F</m> if we have <m>K=F(\alpha_1,\alpha_2,\dots, \alpha_n)</m> for some finite set  <m>\{\alpha_1, \alpha_2,\dots, \alpha_n\}\subseteq K</m>.
			</p>
		</statement>
	</definition>

	<definition xml:id="d_algebraic">
		<title>Algebraic extension</title>
		<statement>
			<p>
				Let <m>K/F</m> be a field extension.
				We say <m>K</m> is <term>algebraic</term> over <m>F</m> if all elements of <m>K</m> are algebraic over <m>F</m>.
			</p>
		</statement>
	</definition>

	<example xml:id="eg_alg_ext">
		<title>Algebraic extensions</title>
		<p>
			The extension <m>\R/\Q</m> is not algebraic, since <m>\pi\in \R</m> is transcendental over <m>\Q</m>.
		</p>

		<p>
			The extension <m>\C/\R</m> is algebraic.
			As we have shown previously, any element <m>a+bi\in \C</m> satisfies the quadratic polynomial <m>x^2+2ax+(a^2+b^2)</m>.
		</p>
	</example>

	<example xml:id="eg_finite_simple_alg">
		<title>Simple extension with algebraic generator</title>
		<statement>
			<p>
				Let <m>K=F(\alpha)</m>, where <m>\alpha</m> is algebraic.
				Prove that <m>K</m> is algebraic over <m>F</m>.
			</p>
		</statement>

		<solution>
			<p>
				According to <xref ref="th_simple_ext"/>, we have <m>\dim_F K=[K:F]=n</m> for some finite <m>n</m>.
				It follows that given any <m>\beta\in K</m>, the set <m>\{\beta^n,\beta^{n-1},\dots, \beta, 1\}</m> is linearly dependent, since it has more than <m>n</m> elements (<xref ref="th_dimension_compendium" text="global"/>,<q>street smarts</q>).
				Thus there is a nontrivial linear combination
				<me>
					a_n\beta^n+a_{n-1}\beta^{n-1}+\cdots +a_1\beta+a_0=0
				</me>.
				In other words, we have <m>f(\beta)=0</m>, where <m>f(x)=\anpoly</m>.
				This proves <m>\beta</m> is algebraic, as desired.
			</p>
		</solution>
	</example>

	<p>
		The main result of this section is <xref ref="th_finite_ext"/>, which both generalizes <xref ref="eg_finite_simple_alg"/> and gives a full characterization of finite extensions in terms of finitely generated and algebraic field extensions.
		First we treat the <xref ref="th_degree_towers" text="custom">tower law</xref>, which will be instrumental in proving <xref ref="th_finite_ext"/>, and is also quite useful in its own right.
	</p>

	<theorem xml:id="th_degree_towers">
		<title>Tower law</title>
		<statement>
			<p>
				Let <m>L/K/F</m> be a tower of (possibly infinite) field extensions.
				<ol>
					<li>
						<p>
							If <m>B_1</m> is a basis of <m>K</m> and <m>B_2</m> is a basis of <m>L</m> as a <m>K</m>-vector space, then the set
							<men xml:id="eq_degree_towers_basis">
								B=\{\alpha\beta\colon \alpha\in B_1, \beta\in B_2\}
							</men>
							of all pairwise products of elements of <m>B_1</m> and <m>B_2</m>
							is a basis of <m>L</m> as an <m>F</m>-vector space.
						</p>
					</li>

					<li>
						<p>
							We have
							<men xml:id="eq_degree_towers_formula">
								[L\colon F]=[L\colon K][K\colon F]
							</men>.
						</p>
					</li>
				</ol>
			</p>
		</statement>
		<proof>
			<title>Proof of (1)</title>
			<p>
				Let <m>B=\{\alpha\beta\colon \alpha\in B_1, \beta\in B_2\}</m>, as in the theorem statement. We will show directly that <m>B</m> is a basis of <m>L</m> as an <m>F</m>-vector space, by showing that it spans and is linearly independent. 
			</p>
			<case>
				<title><m>B</m> spans</title>
				<p>
				 Given any <m>\alpha\in L</m>, since <m>B_2</m> is a <m>K</m>-basis of <m>L</m>, we can write 
				 <me>
					\alpha=c_1\beta_1+c_2\beta_2+\cdots +c_n\beta_n=\sum_{j=1}^nc_j\beta_j
				 </me>
				 for some elements <m>\beta_j\in B_2</m> and scalars <m>c_j\in K</m>. Next since <m>B_1</m> is a basis of <m>K</m> over <m>F</m>, we can find a finite set <m>\{\alpha_1,\alpha_2,\dots, \alpha_m\}\subseteq B_1</m> such that for each <m>1\leq j\leq n</m> we have 
				 <me>
					c_j=d_{1j}\alpha_1+d_{2j}\alpha_2+\cdots +d_{mj}\alpha_m=\sum_{i=1}^md_{ij}\alpha_i
				 </me>
				 for some elements <m>d_{ij}\in F</m>. Substituting these expressions for <m>c_j</m> into the first linear combination above, we conclude that 
				 <md>
					<mrow> \alpha\amp = \sum_{j=1}^nc_j\beta_j </mrow>
					<mrow> \amp = \sum_{j=1}^n (\sum_{i=1}^md_{ij}\alpha_i)\beta_j</mrow>
					<mrow> \amp =\sum_{\substack{1\leq i\leq m\\ 1\leq j\leq n }}d_{ij}\, \alpha_i\, \beta_j </mrow>
				 </md>
				 for some scalars <m>d_{ij}\in F</m> and elements <m>\alpha_i\beta_j\in B</m>. 
				 This shows that every element of <m>L</m> can be written as a <m>F</m>-linear combination of elements of <m>B</m>, and hence that <m>\Span_F B=L</m>. 
				</p>
			</case>
			<case>
				<title><m>B</m> is linearly independent</title>
				<p>
					Assume we have an  <m>F</m>-linear combination 
					<me>
						\sum_{\substack{1\leq i\leq m\\ 1\leq j\leq n }}d_{ij}\alpha_i\, \beta_j=0
					</me>,
					where <m>\alpha_i\in B_1</m>, <m>\beta_j\in B_2</m>, <m>d_{ij}\in F</m> and the elements <m>\alpha_i\beta_j</m> are distinct. Grouping terms, we can re-write this as 
					<me>
						\sum_{j=1}^nc_j\beta_j=0
					</me>,
					where for each <m>1\leq j\leq n</m>, we have 
					<me>
						c_j=\sum_{i=1}^md_{ij}\alpha_j \in K
					</me>. 
					Firstly, since <m>\alpha_i\beta_j\ne \alpha_{i'}\beta_{j'}</m> for all <m>(i,j)\ne (i',j')</m>, it follows easily that <m>\beta_j\ne \beta_{j'}</m> for <m>j\ne j'</m>. Since <m>B_2</m> is linearly independent over <m>K</m>, we conclude that <m>c_j=0</m> for all <m>1\leq j\leq n</m>. But then, since <m>B_1</m> is linearly independent over <m>F</m>, for all <m>1\leq j\leq n</m> we have  
					<me>
						c_j=\sum_{i=1}^md_{ij}\alpha_j=0\implies d_{ij}=0 \text{ for all } 1\leq i\leq m
					</me>.
					We conclude that <m>d_{ij}=0</m> for all <m>1\leq i\leq m</m> and <m>1\leq j\leq n</m>. 
					This proves <m>B</m> is linearly independent over <m>F</m>.
				</p>
				
				</case>
		</proof>
		<proof>
			<title>Proof of (2)</title>
			<p>
				We treat two cases: (a) <m>K/F</m> and <m>L/K</m> are both finite extensions, and (b) at least one of <m>K/F</m> and <m>L/K</m> is an infinite extension.  
			</p>
			<case>
			<title>Case (a)</title>
			<p>
			Assume <m>[K\colon F]=n_1</m> and <m>[L\colon K]=n_2</m>, for positive integers <m>n_1, n_2</m>. By definition we can find bases 
			<md>
				<mrow>B_1 \amp =\{\alpha_1,\alpha_2,\dots, \alpha_{n_1}\}</mrow>
				<mrow>B_2 \amp =\{\beta_1,\beta_2,\dots, \beta_{n_2}\}</mrow>
			</md>
			for <m>K</m> as an <m>F</m>-vector space, and <m>L</m> as a <m>K</m>-vector space, respectively. By statement (1) of this theorem, we conclude that 
			<me>
				B=\{\alpha_i\beta_j\colon 1\leq i\leq n_1, 1\leq j\leq n_2\}
			</me>
			is a basis of <m>L</m> as an <m>F</m>-vector space. It remains only to show that <m>\abs{B}=n_1n_2</m>, since then we have 
			<me>
				[L\colon F]=\dim_F L=\abs{B}=n_1n_2=[K\colon F][L\colon K]=[L\colon K][K\colon F]
			</me>.
			To see that <m>\abs{B}=n_1n_2</m>, we show that the map 
			<md>
				<mrow>B_1\times B_2 \amp \rightarrow B</mrow>
				<mrow>(\alpha, \beta) \amp \mapsto \alpha\beta</mrow>
			</md>
			is a bijection, whence <m>\abs{B}=\abs{B_1}\times \abs{B_2}=n_1n_2</m>. The map is surjective by definition of <m>B</m>. That the map is injective follows from the following chain of implications: 
			<md>
				<mrow> \alpha\beta=\alpha'\beta' \amp \implies \alpha\beta-\alpha'\beta' </mrow>
				<mrow> \amp \implies \beta=\beta' \text{ or } \alpha=\alpha'=0 \amp (B_2 \text{ lin. ind. over } K) </mrow>
				<mrow> \amp\implies \beta=\beta' \amp (B_1 \text{ basis } \implies \alpha\ne 0, \alpha'\ne 0) </mrow>
				<mrow> \amp \implies \alpha=\alpha' \text{ and } \beta=\beta' \amp (\alpha\beta=\alpha'\beta')</mrow>
				<mrow> \amp \implies (\alpha, \beta)=(\alpha', \beta')</mrow>
			</md>.
			</p>
			</case>
			<case>
			<title>Case (b)</title>
			<p>
				Assume first that <m>K/F</m> is infinite. In this case we can find an infinite set <m>S</m> of the form <m>S=\{\alpha_1,\alpha_2,\dots,\}\subseteq K</m> that is linearly independent over <m>F</m>. But <m>S</m> is also a subset of <m>L</m>, and thus <m>L/F</m> has an infinite linearly independent set, making it an infinite extension. 
			</p>
			<p>
			Now assume that <m>L/K</m> is infinite. In this case we can find an infinite set <m>S</m> of the form <m>S=\{\alpha_1,\alpha_2,\dots,\}\subseteq L</m> that is linearly independent over <m>K</m>. But then <m>S</m> is also linearly independent over the smaller field <m>F</m>, since an <m>F</m>-linear combination of elements of <m>S</m> is also a <m>K</m>-linear combination. Thus <m>L/F</m> also has infinite dimension. 
			</p>
			
			</case>
			
		</proof>
	</theorem>

	<remark>
		<title>Tower law</title>
		<p>
			Statement (1) of <xref ref="th_degree_towers"/> is just as important as (2), as it gives us a procedure for building a basis for <m>L/F</m> from bases <m>B_1</m> of <m>L/K</m> and <m>B_2</m> of <m>K/F</m>: namely, we simply take the set of all products of elements in <m>B_1</m> and <m>B_2</m>.
		</p>
	</remark>

	<remark>
		<title>Tower law: infinite extensions</title>
		<p>
			The formula <xref ref="eq_degree_towers_formula"/> is true even when one or more of the field extensions involved is infinite, using the following rules from <q>extended arithmetic</q>:
			<md>
				<mrow>\infty \amp = n\cdot \infty=\infty\cdot n=\infty\cdot \infty \text{ for all positive } n\in \Z </mrow>
				<mrow>\infty \amp\ne m\cdot n \text{ for all positive }  m,n \in \Z  </mrow>
			</md>.
			Equivalently, we can interpret <xref ref="eq_degree_towers_formula"/> as stating that the extension <m>L/F</m> is infinite if and only if <m>L/K</m> is infinite or <m>K/F</m> is infinite.
		</p>
	</remark>

	<corollary xml:id="cor_degree_towers">
		<title>Tower law</title>
		<statement>
			<p>
				<ol>
					<li>
						<p>
							Let <m>L/K/F</m> be a tower of finite field extensions. The integers <m>[K\colon F]</m> and <m>[L\colon K]</m> divide the integer <m>[L\colon F]</m>: <ie/>, we have 
							<me>
								[K\colon F]\, \mid [L\colon F] \text{ and } [L\colon K]\, \mid [L\colon F]
							</me>.
							
						</p>
					</li>

					<li>
						<p>
							Given a tower of extensions
							<me>
								F_1\leq F_2\leq \cdots \leq F_n
							</me>,
							we have
							<me>
								[F_n\colon F_1]=\prod_{k=1}^{n-1}[F_{k+1}\colon F_k]
							</me>.
						</p>
					</li>
				</ol>
			</p>
		</statement>
		<proof>
			<p>
				Statement (1) follows directly from <xref ref="th_degree_towers"/>; statement (2) follows from <xref ref="th_degree_towers"/> by induction. 
			</p>
		</proof>
	</corollary>

	<example xml:id="eg_degree_towers">
		<title>Tower law</title>
		<p>
			Use the tower law to prove that the field extension <m>\Q(\sqrt[3]{2})/\Q</m> has no nontrivial subextension <m>K/\Q</m>: <ie/>, if <m>\Q\leq K\leq \Q(\sqrt[3]{2})</m>, then <m>K=\Q</m> or <m>K=\Q(\sqrt[3]{2})</m>.
		</p>
	</example>

	<theorem xml:id="th_finite_ext">
		<title>Finite extension theorem</title>
		<statement>
			<p>
				Let <m>K/F</m> be a field extension.
				The following statements are equivalent.
				<ol>
					<li>
						<p>
							<m>K/F</m> is finite.
						</p>
					</li>

					<li>
						<p>
							<m>K/F</m> is finitely generated and algebraic.
						</p>
					</li>

					<li>
						<p>
							<m>K=F(\alpha_1,\alpha_2,\dots, \alpha_m)</m>, where <m>\alpha_i\in K</m> is algebraic over <m>F</m>.
							In other words, <m>K</m> is generated over <m>F</m> by finitely many algebraic elements.
						</p>
					</li>
				</ol>
			</p>
		</statement>


		<proof>
			<p>
				We prove the <q>cycle of implications</q> (1)<m>\implies</m>(2)<m>\implies</m>(3)\implies (1)
			</p>

			<case>
				<title>Implication: (1)<m>\implies</m>(2)</title>
				<p>
					Assume <m>K/F</m> is finite, of dimension <m>n</m>.
					<ul>
						<li>
							<p>
								We claim <m>K/F</m> is finitely generated. Let <m>B=\{\alpha_1,\alpha_2,\dots, \alpha_n\}</m> be a basis of <m>K</m> as an <m>F</m>-vector space. Since <m>\Span_F B=K</m>, we have
								<me>
									K=\{c_1\alpha_1+c_2\alpha_2+\cdots +c_n\alpha_n\colon c_i\in F\}
								</me>.
								It follows that <m>K=F(\alpha_1,\alpha_2,\dots, \alpha_n)</m>, and hence is finitely generated (by the elements <m>\alpha_i</m>). Indeed, since <m>F(\alpha_1,\alpha_2,\dots, \alpha_n)</m> is a subfield of <m>K</m> containing <m>F</m> and <m>\alpha_i</m> for all <m>1\leq i\leq n</m>, it must contain all <m>F</m>-linear combinations of the <m>\alpha_i</m>. But then we have  
								<me>
									K=\{c_1\alpha_1+c_2\alpha_2+\cdots +c_n\alpha_n\colon c_i\in F\}\leq F(\alpha_1,\alpha_2,\dots, \alpha_n)\leq K
								</me>,
								and conclude that <m>K=F(\alpha_1,\alpha_2,\dots, \alpha_n)</m>. 
							</p>
						</li>
						<li>
							<p>
								We claim that <m>K/F</m> is algebraic. Take any <m>\beta\in K</m>. Since <m>\dim_F K=n</m>, the set <m>\{\beta^{n+1},\beta^{n},\dots, \beta, 1\}</m>, consisting of <m>n+1</m> elements, is linearly independent. (Street smarts!) Thus there is a nontrivial linear combination 
								<me>
									a_{n+1}\beta^{n+1}+a_{n}\beta^n+\cdots +a_1\beta+1=0
								</me>,
								where <m>a_i\in F</m> for all <m>1\leq i\leq n+1</m>. It follows that the <m>F</m>-polynomial <m>f(x)=a_{n+1}x^{n+1}+a_nx^n+\cdots +a_1x+a_0</m> is nonzero and satisfies <m>f(\beta=0</m>. Thus <m>\beta</m> is algebraic over <m>F</m>, as desired.
							</p>
						</li>
					</ul>
				</p>
			</case>

			<case>
				<title>Implication: (2)<m>\implies</m>(3)</title>
				<p>
					Assume <m>K/F</m> is finitely generated and algebraic. Since <m>K/F</m> is finitely generated, there are elements <m>\alpha_1,\alpha_2,\dots, \alpha_m</m> such that <m>K=F(\alpha_1,\alpha_2,\dots, \alpha_m)</m>. Since <m>K/F</m> is algebraic, each element <m>\alpha_i</m> is algebraic over <m>F</m>. Thus <m>K=F(\alpha_1,\alpha_2,\dots, \alpha_m)</m>, and each <m>\alpha_i</m> is algebraic over <m>F</m>, as desired. 
				</p>
			</case>

			<case>
				<title>Implication: (3)<m>\implies</m>(1)</title>
				<p>
					We will show that any field extension generated by finitely many algebraic elements is finite. The proof will proceed by induction on the number <m>m</m> of generators of the field. 
				</p>
				<p>
					Base step: <m>m=1</m>. Assume <m>K=F(\alpha)</m>, where <m>\alpha</m> is algebraic over <m>F</m>. By <xref ref="th_simple_ext"/>, we have <m>\dim_F K&lt; \infty</m>. Thus <m>K/F</m> is finite.  
				</p>
				<p>
					Induction step: assume <em>any</em> field extension generated over the base field by <m>m</m> algebraic elements is a finite extension. Now suppose we have <m>K=F(\alpha_1,\alpha_2,\dots, \alpha_{m+1})</m>, where each <m>\alpha_i</m> is algebraic over <m>F</m>. If <m>\alpha_i\in F</m> for all <m>i</m>, then <m>F=K</m>, in which case <m>K</m> is finite over <m>F</m>. Otherwise, we may assume without loss of generality that <m>\alpha_1\in K-F</m>. Since <m>\alpha_1</m> is algebraic over <m>F</m>, the extension <m>F(\alpha_1)/F</m> is finite by the base step. Let <m>K'=F(\alpha_1)</m>. We have a tower of fields <m>K/K'/F</m>, and thus by the <xref ref="th_degree_towers" text="custom">tower law</xref>, the extension <m>K/F</m> is finite if and only if <m>K/K'</m> is finite and <m>K'/F</m> is finite. We know already that <m>K'=F(\alpha_1)</m> is finite over <m>F</m>. As for the extension <m>K/K'</m> it is easy to see that 
					<me>
						K=F(\alpha_1,\alpha_2,\dots, \alpha_{m+1})=F(\alpha_1)(\alpha_2,\dots, \alpha_{m+1})=K'(\alpha_2,\dots, \alpha_{m+1})
					</me>.
					Furthermore, since each <m>\alpha_i</m> is satisfies a nonzero polynomial <m>f_i(x)\in F[x]\subseteq K'[x]</m>, we see that each <m>\alpha_i</m> is algebraic over <m>K'</m>. Thus the extension <m>K/K'</m> is generated over <m>K'</m> by the <m>m</m> algebraic elements <m>\alpha_2,\dots, \alpha_{m+1}</m>. By induction <m>K/K'</m> is finite. The <xref ref="th_degree_towers" text="custom">tower law</xref> now implies that <m>K/F</m> is finite. 
				</p>
			</case>
		</proof>
	</theorem>

	<remark>
		<title>Finite extension theorem</title>
		<p>
			As we saw in the proof of <xref ref="th_finite_ext"/>, given a field extension <m>K/F</m> the following implications hold:
			<md>
				<mrow>K/F \text{ finite} \amp\implies K/F \text{ finitely generated} </mrow>
				<mrow>K/F \text{ finite} \amp\implies K/F \text{ algebraic} </mrow>
			</md>.
			On the other hand, neither of these implications goes the other way.
			That is, we have
			<md>
				<mrow>K/F \text{ finite } \hspace{5pt} \amp\not\!\!\!\!\!\!\impliedby K/F \text{ finitely generated} </mrow>
				<mrow>K/F \text{ finite } \hspace{5pt} \amp\not\!\!\!\!\!\!\impliedby K/F \text{ algebraic} </mrow>
			</md>.
			In other words, taken singly, neither of these two properties (finitely generated, algebraic) is strong enough to imply the property of being finite.
			<xref ref="th_finite_ext"/> tells us that the two properties taken together are in fact equivalent to being finite: <ie/>,
			<me>
				K/F \text{ finite } \iff K/F \text{ finitely generated and algebraic}
			</me>.
		</p>
	</remark>
</section>
